src/invariant/PFStepCommon.v
@@ -1,0 +1,195 @@
+Require Import Omega.
+Require Import RelationClasses.
+
+Require Import sflib.
+
+Require Import Axioms.
+Require Import Basic.
+Require Import DataStructure.
+Require Import DenseOrder.
+Require Import Time.
+Require Import Event.
+Require Import Language.
+Require Import View.
+Require Import Cell.
+Require Import Memory.
+Require Import TView.
+Require Import Local.
+Require Import Thread.
+
+Require Import PromiseConsistent.
+
+Set Implicit Arguments.
+
+
+Module PFStepCommon.
+  Inductive sim_promises (promises_src promises_tgt: Memory.t): Prop :=
+  | sim_promises_intro
+      (SOUND: forall loc from to msg_src
+                (GET_SRC: Memory.get loc to promises_src = Some (from, msg_src)),
+          exists msg_tgt,
+            <<GET_TGT: Memory.get loc to promises_tgt = Some (from, msg_tgt)>>)
+      (COMPLETE: forall loc from to msg
+                   (GET_TGT: Memory.get loc to promises_tgt = Some (from, msg)),
+          <<GET_SRC: Memory.get loc to promises_src = Some (from, Message.half)>>)
+  .
+
+  Inductive sim_local (lc_src lc_tgt: Local.t): Prop :=
+  | sim_local_intro
+      (TVIEW: TView.le lc_src.(Local.tview) lc_tgt.(Local.tview))
+      (PROMISES: sim_promises lc_src.(Local.promises) lc_tgt.(Local.promises))
+  .
+
+  Inductive sim_message: forall (msg_src msg_tgt: Message.t), Prop :=
+  | sim_message_full
+      val released_src released_tgt
+      (RELEASED: View.opt_le released_src released_tgt):
+      sim_message (Message.full val released_src) (Message.full val released_tgt)
+  | sim_message_half:
+      sim_message Message.half Message.half
+  .
+  Hint Constructors sim_message.
+
+  Program Instance sim_message_PreOrder: PreOrder sim_message.
+  Next Obligation.
+    ii. destruct x; econs; refl.
+  Qed.
+  Next Obligation.
+    ii. inv H; inv H0; econs. etrans; eauto.
+  Qed.
+
+  Definition vals_incl (mem1 mem2: Memory.t): Prop :=
+    forall loc from to val released
+      (GET1: Memory.get loc to mem1 = Some (from, Message.full val released)),
+    exists f t v r,
+      <<GET2: Memory.get loc t mem2 = Some (f, Message.full v r)>>.
+
+  Program Instance vals_incl_PreOrder: PreOrder vals_incl.
+  Next Obligation.
+    ii. eauto.
+  Qed.
+  Next Obligation.
+    ii. exploit H; eauto. i. des. eauto.
+  Qed.
+
+  Lemma sim_promises_get_src
+        promises_src promises_tgt
+        loc from to msg_src
+        (PROMISES: sim_promises promises_src promises_tgt)
+        (GET_SRC: Memory.get loc to promises_src = Some (from, msg_src)):
+    exists msg_tgt,
+      <<GET_TGT: Memory.get loc to promises_tgt = Some (from, msg_tgt)>> /\
+      <<MSG: msg_src = Message.half>>.
+  Proof.
+    inv PROMISES.
+    exploit SOUND; eauto. i. des.
+    exploit COMPLETE; eauto. i. des.
+    rewrite GET_SRC in x. inv x.
+    esplits; eauto.
+  Qed.
+
+
+  (* lemmas on step *)
+
+  Lemma fence_step
+        lc1_src sc1_src mem1_src
+        lc1_tgt sc1_tgt mem1_tgt ordr ordw lc2_tgt sc2_tgt
+        (LOCAL1: sim_local lc1_src lc1_tgt)
+        (SC1: TimeMap.le sc1_src sc1_tgt)
+        (WF1_SRC: Local.wf lc1_src mem1_src)
+        (WF1_TGT: Local.wf lc1_tgt mem1_tgt)
+        (STEP_TGT: Local.fence_step lc1_tgt sc1_tgt ordr ordw lc2_tgt sc2_tgt):
+    exists lc2_src sc2_src,
+      <<STEP_SRC: Local.fence_step lc1_src sc1_src ordr ordw lc2_src sc2_src>> /\
+      <<LOCAL2: sim_local lc2_src lc2_tgt>> /\
+      <<SC2: TimeMap.le sc2_src sc2_tgt>>.
+  Proof.
+    esplits.
+    - econs; eauto. ii. inv LOCAL1.
+      exploit sim_promises_get_src; eauto. i. des. subst. ss.
+    - inv STEP_TGT. inv LOCAL1. econs; eauto. ss.
+      eapply TViewFacts.write_fence_tview_mon; try refl; ss.
+      + eapply TViewFacts.read_fence_tview_mon; try refl; ss.
+        apply WF1_TGT.
+      + eapply TViewFacts.read_fence_future; apply WF1_SRC.
+    - inv STEP_TGT. inv LOCAL1.
+      eapply TViewFacts.write_fence_sc_mon; try refl; ss.
+      eapply TViewFacts.read_fence_tview_mon; try refl; ss.
+      apply WF1_TGT.
+  Qed.
+
+
+  (* existence of sim_promises *)
+
+  Inductive sim_promises_aux (dom: list (Loc.t * Time.t)) (promises_src promises_tgt: Memory.t): Prop :=
+  | sim_promises_aux_intro
+      (SOUND: forall loc from to msg_src
+                (GET_SRC: Memory.get loc to promises_src = Some (from, msg_src)),
+          List.In (loc, to) dom /\
+          exists msg_tgt, Memory.get loc to promises_tgt = Some (from, msg_tgt))
+      (COMPLETE: forall loc from to msg_tgt
+                   (IN: List.In (loc, to) dom)
+                   (GET_TGT: Memory.get loc to promises_tgt = Some (from, msg_tgt)),
+          Memory.get loc to promises_src = Some (from, Message.half))
+  .
+
+  Lemma sim_promises_aux_exists
+        dom promises_tgt
+        (BOT: Memory.bot_none promises_tgt):
+    exists promises_src,
+      sim_promises_aux dom promises_src promises_tgt.
+  Proof.
+    induction dom.
+    { exists Memory.bot. econs; ss. i.
+      rewrite Memory.bot_get in *. ss. }
+    des. destruct a as [loc to]. inv IHdom.
+    destruct (Memory.get loc to promises_tgt) as [[from msg]|] eqn:GETT; cycle 1.
+    { exists promises_src. econs; i.
+      - exploit SOUND; eauto. i. des.
+        esplits; eauto. econs 2. ss.
+      - inv IN.
+        + inv H. congr.
+        + exploit COMPLETE; eauto.
+    }
+    destruct (Memory.get loc to promises_src) as [[from_src msg_src]|] eqn:GETS.
+    - exploit SOUND; eauto. i. des.
+      rewrite GETT in x0. inv x0.
+      exists promises_src. econs; i.
+      + exploit SOUND; try exact GET_SRC. i. des.
+        esplits; eauto. econs 2. ss.
+      + inv IN.
+        * inv H. exploit COMPLETE; try exact GET_TGT; eauto.
+        * exploit COMPLETE; try exact GET_TGT; eauto.
+    - exploit (@Memory.add_exists promises_src loc from to Message.half); ii.
+      { exploit SOUND; eauto. i. des.
+        exploit Memory.get_disjoint; [exact GETT|exact x1|..].
+        i. des; eauto; congr. }
+      { exploit Memory.get_ts; try exact GETT. i. des; ss.
+        subst. rewrite BOT in GETT. ss. }
+      { econs. }
+      des. exists mem2. econs; i.
+      + revert GET_SRC. erewrite Memory.add_o; eauto. condtac; ss.
+        * i. inv GET_SRC. des. subst. split; eauto.
+        * i. guardH o. exploit SOUND; eauto. i. des.
+          split; eauto.
+      + inv IN.
+        * inv H. rewrite GETT in GET_TGT. inv GET_TGT.
+          exploit Memory.add_get0; eauto. i. des. ss.
+        * exploit COMPLETE; eauto. i.
+          erewrite Memory.add_o; eauto. condtac; ss.
+          des. subst. rewrite GETT in GET_TGT. inv GET_TGT. ss.
+  Qed.
+
+  Lemma sim_promises_exists
+        promises_tgt
+        (BOT: Memory.bot_none promises_tgt):
+    exists promises_src,
+      sim_promises promises_src promises_tgt.
+  Proof.
+    destruct (Memory.finite promises_tgt).
+    exploit (@sim_promises_aux_exists x promises_tgt); ss. i. des.
+    exists promises_src. inv x1. econs; i.
+    - exploit SOUND; eauto. i. des. eauto.
+    - exploit COMPLETE; eauto.
+  Qed.
+End PFStepCommon.
